SSAValues.thy
@@ -10,12 +10,8 @@ lemma memory_\<alpha>_eq[simp]: "memory_\<alpha> (vs,s,h) = memory_\<alpha> (vs'
     by (cases x; simp)
   done
 
-lemma ssa_set_\<alpha>_update_eq[simp]:
-  "ssa_set_\<alpha> (ssa (Mapping.update n v m) (insert n a), s, h) = (ssa_set_\<alpha> (ssa m a, s, h))(n := True)"
-  by (auto simp: fun_eq_iff)
-
 lemma ssa_\<alpha>_update_eq[simp]:
-  "ssa_\<alpha> (ssa (Mapping.update n v m) (insert n a), s, h) = (ssa_\<alpha> (ssa m a, s, h))(ssa_val n := Some v)"
+  "ssa_\<alpha> (Mapping.update n v vs, s, h) = (ssa_\<alpha> (vs, s, h))(ssa_val n := Some v)"
   apply (auto simp: fun_eq_iff split: llvm_value_ref.split)
   subgoal for x by (cases x; simp)
   done
@@ -26,27 +22,13 @@ section "Lemmas"
 named_theorems ssa_value_intro
 
 lemma wp_set_ssa_value_intro[THEN consequence, ssa_value_intro]:
-  assumes "\<not>ssa_set_\<alpha> (vs,s,h) n"
-  shows "wp (set_ssa_value vs n v) (\<lambda>vs'. ssa_set_\<alpha> (vs',s,h) = (ssa_set_\<alpha> (vs,s,h))(n := True) \<and> ssa_\<alpha> (vs',s,h) = (ssa_\<alpha> (vs,s,h))(ssa_val n := Some v) \<and> memory_\<alpha> (vs',s,h) = memory_\<alpha> (vs,s,h))"
-  using assms
-  by (cases vs; simp; intro wp_intro; simp)
+  "wp (return (set_ssa_value vs n v,s,h)) (\<lambda>s'. ssa_\<alpha> s' = (ssa_\<alpha> (vs,s,h))(ssa_val n := Some v) \<and> memory_\<alpha> s' = memory_\<alpha> (vs,s,h))"
+  unfolding set_ssa_value_def
+  by (intro wp_intro wp_return_intro; simp)
 
 lemma wp_set_ssa_intro[THEN consequence, wp_intro]:
-  assumes "\<not>ssa_set_\<alpha> s n"
-  shows "wp (set_ssa s n v) (\<lambda>s'. ssa_set_\<alpha> s' = (ssa_set_\<alpha> s)(n := True) \<and> ssa_\<alpha> s' = (ssa_\<alpha> s)(ssa_val n := Some v) \<and> memory_\<alpha> s' = memory_\<alpha> s)"
-  unfolding set_ssa_def
-  using assms
-  by (intro wp_intro ssa_value_intro wp_return_intro; simp)
-
-
-lemma wp_reset_ssa_assigned_intro[THEN consequence, wp_intro]:
-  shows "wp (return (reset_ssa_assigned s)) (\<lambda>s'. ssa_set_\<alpha> s' = (\<lambda>_. False) \<and> ssa_\<alpha> s' = ssa_\<alpha> s \<and> memory_\<alpha> s' = memory_\<alpha> s)"
-  apply (cases s; simp)
-  apply (intro wp_intro wp_return_intro; auto; rule ext)
-  subgoal for vs s h n by (cases vs; cases n; simp)
-  subgoal for vs s h n by (cases vs; cases n; simp)
-  subgoal for vs s h a by (cases vs; cases a; simp)
-  done
+  shows "wp (return (set_ssa s n v)) (\<lambda>s'. ssa_\<alpha> s' = (ssa_\<alpha> s)(ssa_val n := Some v) \<and> memory_\<alpha> s' = memory_\<alpha> s)"
+  by (cases s; simp; intro wp_intro ssa_value_intro; simp)
 
 
 lemma wp_get_ssa_value_intro[THEN consequence, ssa_value_intro]:
